\documentclass{article}
\usepackage{latexsym,amsfonts,amssymb,amsthm,amsmath}
\usepackage[margin=0.5in]{geometry}
\title{Homework 1}

\begin{document}

\section*{Question 1}
\[ABC=IC= AI\]
So \[A=C\]
\section*{Question2} 
\begin{align*}
\text{tr}(AB) &= \sum_{i=1}^{n} (AB)_{ii} \\
              &= \sum_{i=1}^{n} \sum_{k=1}^{p} A_{ik} B_{ki} \\
              &= \sum_{k=1}^{p} \sum_{i=1}^{n} B_{ki} A_{ik} \\
              &= \sum_{k=1}^{p} (BA)_{kk} \\
              &= \text{tr}(BA).
\end{align*}

\section*{Question 3}

Suppose \( \mathit{v} \) is an eigenvector of both \( A \) and \( B \)
\[
A \mathit{v} = \lambda \mathit{v}, \quad B \mathit{v} = \mu \mathit{}{v}
\]

\subsection*{For \( AB \):}
\[
AB \mathit{v} = A (B \mathit{v}) = A (\mu \mathit{v}) = \mu (A \mathit{v}) = \mu (\lambda \mathit{v}) = (\lambda \mu) \mathit{v}
\]

\subsection*{For \( BA \):}
\[
BA \mathit{v} = B (A \mathit{v}) = B (\lambda \mathit{v}) = \lambda (B \mathit{v}) = \lambda (\mu \mathit{v}) = (\lambda \mu) \mathit{v}
\]

So, \( \mathit{v} \) is an eigenvector of both \( AB \) and \( BA \) with eigenvalue \( \lambda \mu \).

\section*{Question 4}

   \[ A^\top A v = \lambda v, \]
  Let \[ \mu = Av, \]
 Then,   \begin{align*}
    A A^\top \mu &= A A^\top (Av) \\
    &= A (A^\top A) v \\
    &= A (\lambda v) \\
     &= \lambda (A v) \\
    &= \lambda \mu \\   
\end{align*}
So,  \[A A^\top \mu = \lambda \mu \]
\section*{Question 5}

\begin{align*}   
f_{X,Y}(x, y)  &= \frac{1}{\sqrt{2\pi \sigma^2}} \exp\left(-\frac{(x - y)^2}{2\sigma^2}\right) \cdot \frac{1}{\sqrt{2\pi}} \exp\left(-\frac{y^2}{2}\right) \\
&= \frac{1}{2\pi \sigma} \exp\left(-\frac{(x - y)^2}{2\sigma^2} - \frac{y^2}{2}\right) \\
\end{align*}



\begin{align*}
f_X(x) &= \int_{-\infty}^{\infty} f_{X,Y}(x, y) \, dy \\
&= \frac{1}{2\pi\sigma} \int_{-\infty}^{\infty} \exp \left(-\frac{(x - y)^2}{2\sigma^2} - \frac{y^2}{2}\right) \, dy \\
&= \frac{1}{2\pi\sigma} \int_{-\infty}^{\infty} \exp \left(-\frac{x^2}{2\sigma^2} + \frac{xy}{\sigma^2} - \frac{y^2}{2\sigma^2} - \frac{y^2}{2}\right) \, dy \\
&= \frac{1}{2\pi\sigma} \int_{-\infty}^{\infty} \exp \left(-\frac{x^2}{2\sigma^2} + \frac{xy}{\sigma^2} - \frac{y^2}{2} \left(\frac{\sigma^2 + 1}{\sigma^2}\right)\right) \, dy \\
&= \frac{1}{2\pi\sigma} \exp\left(-\frac{x^2}{2(\sigma^2 + 1)}\right) \int_{-\infty}^{\infty} \exp \left(-\frac{\sigma^2 + 1}{2\sigma^2} \left(y - \frac{x}{\sigma^2 + 1}\right)^2\right) \, dy \\
&\text{Let}  z = y - \frac{x}{\sigma^2 + 1}, \quad dy = dz \\
&= \frac{1}{2\pi\sigma} \exp\left(-\frac{x^2}{2(\sigma^2 + 1)}\right) \int_{-\infty}^{\infty} \exp\left(-\frac{\sigma^2 + 1}{2\sigma^2} z^2\right) \, dz \\
&= \frac{1}{2\pi\sigma} \exp\left(-\frac{x^2}{2(\sigma^2 + 1)}\right) \sqrt{\frac{2\pi\sigma^2}{\sigma^2 + 1}} \\
&= \frac{1}{\sqrt{2\pi(1 + \sigma^2)}} \exp\left(-\frac{x^2}{2(1 + \sigma^2)}\right).
\end{align*}

So,
\(
X \sim N(0, 1 + \sigma^2)
\)


\begin{align*}
    f_{Y|X}(y|x) &= \frac{f_{X|Y}(x|y) \cdot f_Y(y)}{f_X(x)} \\
    &= \frac{\left(\frac{1}{\sqrt{2\pi \sigma^2}} \exp\left(-\frac{(x - y)^2}{2\sigma^2}\right)\right) \cdot \left(\frac{1}{\sqrt{2\pi}} \exp\left(-\frac{y^2}{2}\right)\right)}{\frac{1}{\sqrt{2\pi (\sigma^2 + 1)}} \exp\left(-\frac{x^2}{2(\sigma^2 + 1)}\right)} \\
    &= \frac{\sqrt{2\pi (\sigma^2 + 1)}}{\sqrt{2\pi \sigma^2} \cdot \sqrt{2\pi}} \exp\left(-\frac{(x - y)^2}{2\sigma^2} - \frac{y^2}{2} + \frac{x^2}{2(\sigma^2 + 1)}\right) \\
    &= \frac{1}{\sqrt{2\pi \frac{\sigma^2}{\sigma^2 + 1}}} \exp\left(-\frac{\left(y - \frac{\sigma^2}{\sigma^2 + 1} x\right)^2}{2 \frac{\sigma^2}{\sigma^2 + 1}}\right) \\
    Y | X \sim N\left(\frac{\sigma^2}{\sigma^2 + 1} x, \frac{\sigma^2}{\sigma^2 + 1}\right)
\end{align*}

\section*{Question 6}

\[
f_X(x) = \int_{-\infty}^{\infty} \frac{|y|}{\sqrt{2 \pi \sigma^2}} \exp\left(-\frac{y^2 x^2}{2 \sigma^2}\right) \frac{1}{\sqrt{2 \pi}} \exp\left(-\frac{y^2}{2}\right) \, dy
\]


\[
f_X(x) = \frac{1}{2 \pi \sqrt{\sigma^2}} \int_{-\infty}^{\infty} |y| \exp\left(-\frac{y^2 (x^2 + \sigma^2)}{2 \sigma^2}\right) \, dy
=\frac{1}{\pi \sqrt{\sigma^2}} \int_{0}^{\infty} y \exp(-a y^2) \, dy, \quad a = \frac{x^2 + \sigma^2}{2 \sigma^2}
\]

Let \( u = a y^2 \), \(du=2ady\)

\begin{align*}
    f_X(x) &= \frac{1}{\pi \sqrt{\sigma^2}} \cdot \frac{1}{2a} \int_{0}^{\infty} \exp(-u) \, du \\ 
    &= \frac{1}{\pi \sqrt{\sigma^2}} \cdot \frac{1}{2a} [-\exp(-u)]_{0}^{\infty}\\ 
    &= \frac{1}{\pi \sqrt{\sigma^2}} \cdot \frac{1}{2a}\\
    &= \frac{1}{\pi \sqrt{\sigma^2}} \cdot \frac{1}{\frac{x^2 + \sigma^2}{ \sigma^2}}\\
    &= \frac{1}{\pi \sqrt{\sigma^2}} \cdot \frac{\sigma^2}{x^2 + \sigma^2}\\
    &= \frac{\sigma}{\pi (\sigma^2 + x^2)} \\
\end{align*}

Since $Z= Y^2$ then Z $\sim \chi^2_1$
\begin{align*}
f_{X|Z}(x|z) &= \frac{1}{\sqrt{2 \pi \frac{\sigma^2}{z}}} \exp\left(-\frac{x^2}{2 \frac{\sigma^2}{z}}\right) \\
&= \frac{\sqrt{z}}{\sqrt{2 \pi \sigma^2}} \exp\left(-\frac{z x^2}{2 \sigma^2}\right)
\end{align*}

\begin{align*}
f_{Z|X}(z|x) &= \frac{f_{X|Z}(x|z) f_Z(z)}{f_X(x)} \\
&= \frac{\left(\frac{\sqrt{z}}{\sqrt{2 \pi \sigma^2}} \exp\left(-\frac{z x^2}{2 \sigma^2}\right)\right) \left(\frac{1}{\sqrt{2\pi z}} \exp\left(-\frac{z}{2}\right)\right)}{\frac{\sigma}{\pi (\sigma^2 + x^2)}} \\
&= \frac{1}{2 \pi \sigma} \exp\left(-z \left(\frac{x^2}{2 \sigma^2} + \frac{1}{2}\right)\right) \cdot \frac{\pi (\sigma^2 + x^2)}{\sigma} \\
&= \frac{(\sigma^2 + x^2)}{2 \sigma^2} \exp\left(-z \left(\frac{x^2}{2 \sigma^2} + \frac{1}{2}\right)\right)
\end{align*}


\section*{Question 7}
\[
\begin{pmatrix}
1 & 0 & 0 \\
1 & 1 & 0 \\
1 & 0 & 1
\end{pmatrix}
\begin{pmatrix}
Z_1 \\
Z_2 \\
Z_3
\end{pmatrix}
= \begin{pmatrix}
    Z_1 \\
    Z_1+Z_2\\
    Z_1+Z_3
\end{pmatrix}
\]

\[
\begin{aligned}
Y_1 &= Z_1, \\
Y_2 &= Z_1 + Z_2, \\
Y_3 &= Z_1 + Z_3.
\end{aligned}
\]
\

\begin{align*}
&Y_2 = Z_1 + Z_2 = Y_1 + Z_2 \\
&Y_3 = Z_1 + Z_3 = Y_1 + Z_3 \\
&\mathbb{E}[Y_2 \mid Y_1] = \mathbb{E}[Y_1 + Z_2 \mid Y_1] = Y_1 + \mathbb{E}[Z_2] = Y_1 \\
&\mathbb{E}[Y_3 \mid Y_1] = \mathbb{E}[Y_1 + Z_3 \mid Y_1] = Y_1 + \mathbb{E}[Z_3] = Y_1 \\
\end{align*}


\[Y_2 Y_3 
= (Y_1 + Z_2)(Y_1 + Z_3) = Y_1^2 + Y_1 Z_3 + Y_1 Z_2 + Z_2 Z_3, \]

\begin{align*}
\mathbb{E}[Y_2 Y_3 \mid Y_1] 
&= \mathbb{E}[Y_1^2 + Y_1 Z_3 + Y_1 Z_2 + Z_2 Z_3 \mid Y_1], \\
&= Y_1^2 + Y_1 \mathbb{E}[Z_3 \mid Y_1] + Y_1 \mathbb{E}[Z_2 \mid Y_1] + \mathbb{E}[Z_2 Z_3 \mid Y_1], \\
&= Y_1^2 + Y_1 (0) + Y_1 (0) + \mathbb{E}[Z_2 Z_3]\\
&= Y_1^2 + 0 + 0 + 0 \\
&= Y_1^2 \\
\end{align*}

\begin{align*}
\text{Cov}(Y_2, Y_3 \mid Y_1) 
&= \mathbb{E}[Y_2 Y_3 \mid Y_1] - \mathbb{E}[Y_2 \mid Y_1] \mathbb{E}[Y_3 \mid Y_1] \\
&= Y_1^2 - (Y_1)(Y_1)\\
&= Y_1^2 - Y_1^2 \\
&= 0
\end{align*}

$Y_2$  and  $Y_3$ are independent given $Y_1$

\section*{Question 8}
\[
\mathbf{Y} = 
\begin{pmatrix} 
0 & 1 & 0 \\ 
1 & 1 & 0 \\ 
0 & 1 & 1 
\end{pmatrix} 
\begin{pmatrix} 
Z_1 \\ 
Z_2 \\ 
Z_3 
\end{pmatrix} 
= 
\begin{pmatrix}
Z_2 \\
Z_1 + Z_2 \\
Z_2 + Z_3
\end{pmatrix}.
\]

\[
\mathbf{X} = 
\begin{pmatrix} 
0 & 0 & 1 \\ 
1 & 0 & 1 \\ 
0 & -1 & 1 
\end{pmatrix} 
\begin{pmatrix} 
Z_1 \\ 
Z_2 \\ 
Z_3 
\end{pmatrix} 
= 
\begin{pmatrix}
Z_3 \\
Z_1 + Z_3 \\
-Z_2 + Z_3
\end{pmatrix}.
\]
Since $Z_i$ is stand normal, so $\mathbb{E}(X)=0, \mathbb{E}(Y)=0$
\[
\Sigma_{Y} =
\begin{pmatrix} 
0 & 1 & 0 \\ 
1 & 1 & 0 \\ 
0 & 1 & 1 
\end{pmatrix} 
\begin{pmatrix} 
0 & 1 & 0 \\ 
1 & 1 & 1 \\ 
0 & 0 & 1 
\end{pmatrix} 
= \begin{pmatrix} 
1 & 1 & 1 \\ 
1 & 2 & 1 \\ 
1 & 1 & 2 
\end{pmatrix}
\]

\[
\Sigma_{X}=
\begin{pmatrix} 
0 & 0 & 1 \\ 
1 & 0 & 1 \\ 
0 & -1 & 1 
\end{pmatrix} 
\begin{pmatrix} 
0 & 1 & 0 \\ 
0 & 0 & -1 \\ 
1 & 1 & 1 
\end{pmatrix} 
= \begin{pmatrix} 
1 & 1 & 1 \\ 
1 & 2 & 1 \\ 
1 & 1 & 2 
\end{pmatrix}
\]

Since X and Y have the same covariance matrices. 
Also, they have the same mean. X and Y have the
same distribution.

For X and Y, they are different linear transforms of Z, they are not equal as random variables.

 




\end{document}
